verity/artifacts/sphincs-kernel/MerkleKernel.yul
@@ -254,52 +254,61 @@ object "MerkleKernel" {
                         let sibling3 := calldataload(132)
                         let directions := calldataload(164)
                         let stored := sload(0)
-                        let sibling0OnLeft := iszero(eq(and(directions, 1), 0))
-                        let sibling1OnLeft := iszero(eq(and(shr(1, directions), 1), 0))
-                        let sibling2OnLeft := iszero(eq(and(shr(2, directions), 1), 0))
-                        let sibling3OnLeft := iszero(eq(and(shr(3, directions), 1), 0))
-                        let level0 := 0
                         {
-                            let __ite_cond := sibling0OnLeft
+                            let __ite_cond := iszero(eq(shr(4, directions), 0))
                             if __ite_cond {
-                                level0 := add(mul(sibling0, 65537), add(mul(leaf, 257), 97))
+                                mstore(0, 0)
+                                return(0, 32)
                             }
                             if iszero(__ite_cond) {
-                                level0 := add(mul(leaf, 65537), add(mul(sibling0, 257), 97))
+                                let sibling0OnLeft := iszero(eq(and(directions, 1), 0))
+                                let sibling1OnLeft := iszero(eq(and(shr(1, directions), 1), 0))
+                                let sibling2OnLeft := iszero(eq(and(shr(2, directions), 1), 0))
+                                let sibling3OnLeft := iszero(eq(and(shr(3, directions), 1), 0))
+                                let level0 := 0
+                                {
+                                    let __ite_cond := sibling0OnLeft
+                                    if __ite_cond {
+                                        level0 := add(mul(sibling0, 65537), add(mul(leaf, 257), 97))
+                                    }
+                                    if iszero(__ite_cond) {
+                                        level0 := add(mul(leaf, 65537), add(mul(sibling0, 257), 97))
+                                    }
+                                }
+                                let level1 := 0
+                                {
+                                    let __ite_cond := sibling1OnLeft
+                                    if __ite_cond {
+                                        level1 := add(mul(sibling1, 65537), add(mul(level0, 257), 97))
+                                    }
+                                    if iszero(__ite_cond) {
+                                        level1 := add(mul(level0, 65537), add(mul(sibling1, 257), 97))
+                                    }
+                                }
+                                let level2 := 0
+                                {
+                                    let __ite_cond := sibling2OnLeft
+                                    if __ite_cond {
+                                        level2 := add(mul(sibling2, 65537), add(mul(level1, 257), 97))
+                                    }
+                                    if iszero(__ite_cond) {
+                                        level2 := add(mul(level1, 65537), add(mul(sibling2, 257), 97))
+                                    }
+                                }
+                                let candidate := 0
+                                {
+                                    let __ite_cond := sibling3OnLeft
+                                    if __ite_cond {
+                                        candidate := add(mul(sibling3, 65537), add(mul(level2, 257), 97))
+                                    }
+                                    if iszero(__ite_cond) {
+                                        candidate := add(mul(level2, 65537), add(mul(sibling3, 257), 97))
+                                    }
+                                }
+                                mstore(0, eq(candidate, stored))
+                                return(0, 32)
                             }
                         }
-                        let level1 := 0
-                        {
-                            let __ite_cond := sibling1OnLeft
-                            if __ite_cond {
-                                level1 := add(mul(sibling1, 65537), add(mul(level0, 257), 97))
-                            }
-                            if iszero(__ite_cond) {
-                                level1 := add(mul(level0, 65537), add(mul(sibling1, 257), 97))
-                            }
-                        }
-                        let level2 := 0
-                        {
-                            let __ite_cond := sibling2OnLeft
-                            if __ite_cond {
-                                level2 := add(mul(sibling2, 65537), add(mul(level1, 257), 97))
-                            }
-                            if iszero(__ite_cond) {
-                                level2 := add(mul(level1, 65537), add(mul(sibling2, 257), 97))
-                            }
-                        }
-                        let candidate := 0
-                        {
-                            let __ite_cond := sibling3OnLeft
-                            if __ite_cond {
-                                candidate := add(mul(sibling3, 65537), add(mul(level2, 257), 97))
-                            }
-                            if iszero(__ite_cond) {
-                                candidate := add(mul(level2, 65537), add(mul(sibling3, 257), 97))
-                            }
-                        }
-                        mstore(0, eq(candidate, stored))
-                        return(0, 32)
                     }
                     default {
                         revert(0, 0)
